Updated Timeout example

ft_tests/Timeout.bpl
@@ -21,6 +21,9 @@ var AT#intlst: List int;
 
 function AT#Min(x:int, y: int): int { if x <= y then x else y }
 
+// -- Types and global variables ---------------------------------
+type SeqType = <a>[Chan a][int]int;
+var Seq: SeqType;
 
 // ---------------------------------------------------------------
 // -- End of prelude ---------------------------------------------
@@ -30,42 +33,53 @@ axiom Base#L == 1;
 procedure Rep#anon$0#0()
   modifies C, R, M, St;
 {
-  var IV#in#0: int;
+  var in: Chan (int);
+  var out: Chan (int);
   assume true;
   assume true;
 }
 procedure Split#anon$1#1()
   modifies C, R, M, St;
 {
-  var IV#in#0: int;
+  var in: Chan (int);
+  var out1: Chan (int);
+  var out2: Chan (int);
   assume true;
   assume true;
 }
 procedure Adjudicator#normal#2()
   modifies C, R, M, St;
 {
-  var IV#x1#0: int;
-  var IV#x2#0: int;
-  var IV#c_in#0: int;
+  var x1: Chan (int);
+  var x2: Chan (int);
+  var c_in: Chan (int);
+  var y: Chan (int);
+  var c_out: Chan (int);
   assume true;
-  assume (IV#x1#0 == IV#x2#0) && (IV#x1#0 == IV#c_in#0);
+  assume (M[x1][0] == M[x2][0]) && (M[x1][0] == M[c_in][0]);
   assume true;
 }
 procedure Adjudicator#timeout#3()
   modifies C, R, M, St;
 {
-  var IV#x2#0: int;
-  var IV#c_in#0: int;
+  var x1: Chan (int);
+  var x2: Chan (int);
+  var c_in: Chan (int);
+  var y: Chan (int);
+  var c_out: Chan (int);
   assume true;
   assume true;
 }
 procedure Adjudicator#readoff#4()
   modifies C, R, M, St;
 {
-  var IV#x1#0: int;
-  var IV#c_in#0: int;
+  var x1: Chan (int);
+  var x2: Chan (int);
+  var c_in: Chan (int);
+  var y: Chan (int);
+  var c_out: Chan (int);
   assume true;
-  assume IV#x1#0 < IV#c_in#0;
+  assume M[x1][0] < M[c_in][0];
   assume true;
 }
 procedure Net#init#5()
@@ -104,7 +118,8 @@ procedure Net#anon$2#entry#6()
 {
   var ActionPH#y1: int;
   var ActionPH#y2: int;
-  assume L[Net#a] == (2 * Base#L);
+  var ActionPH#y3: int;
+  assume L[Net#a] == (3 * Base#L);
   assume R[Net#a] == 0;
   assume C[Net#a] == 0;
   assume R[Net#b] == 0;
@@ -121,7 +136,7 @@ procedure Net#anon$2#entry#6()
   assume C[Net#g] == 0;
   C[Net#f] := C[Net#f] + 1;
   assume M[Net#f][R[Net#f]] == 0;
-  assume (M[Net#a][0] == 0) && (M[Net#a][1] == 1);
+  assume (M[Net#a][0] == 0) && (M[Net#a][1] == 1) && (M[Net#a][2] == 2);
   assume 0 <= R[Net#a];
   assume 0 <= C[Net#a];
   assume (R[Net#a] + C[Net#a]) <= L[Net#a];
@@ -138,7 +153,7 @@ procedure Net#anon$2#entry#6()
   assume 0 <= R[Net#g];
   assume 0 <= C[Net#g];
   assume R[Net#g] == 0;
-  assert {:msg "  Channel invariant might not hold on action entry (#16)"} (M[Net#a][0] == 0) && (M[Net#a][1] == 1);
+  assert {:msg "  Channel invariant might not hold on action entry (#16)"} (M[Net#a][0] == 0) && (M[Net#a][1] == 1) && (M[Net#a][2] == 2);
   assert {:msg "  Channel invariant might not hold on action entry (#17)"} R[Net#a] == (R[Net#b] + C[Net#b]);
   assert {:msg "  Channel invariant might not hold on action entry (#18)"} R[Net#a] == (R[Net#c] + C[Net#c]);
   assert {:msg "  Channel invariant might not hold on action entry (#19)"} R[Net#b] == (R[Net#d] + C[Net#d]);
@@ -155,28 +170,13 @@ procedure Net#anon$2#entry#6()
   assert {:msg "  Channel invariant might not hold on action entry (#24)"} (forall idx$: int :: 
     (0 <= idx$) && (idx$ < (R[Net#e] + C[Net#e])) ==> (M[Net#e][idx$] == M[Net#c][idx$])
   );
-  assert {:msg "  40.3: Channel invariant might not hold on action entry (#25)"} (R[Net#a] + C[Net#a]) <= 2;
-  assert {:msg "  41.3: Channel invariant might not hold on action entry (#26)"} (forall i: int :: 
-    (1 <= i) && (i < (R[Net#a] + C[Net#a])) ==> (M[Net#a][i] > M[Net#a][i - 1])
-  );
-  assert {:msg "  42.3: Channel invariant might not hold on action entry (#27)"} (forall i: int :: 
-    (1 <= i) && (i < (R[Net#b] + C[Net#b])) ==> (M[Net#b][i] > M[Net#b][i - 1])
-  );
-  assert {:msg "  43.3: Channel invariant might not hold on action entry (#28)"} (forall i: int :: 
-    (1 <= i) && (i < (R[Net#c] + C[Net#c])) ==> (M[Net#c][i] > M[Net#c][i - 1])
-  );
-  assert {:msg "  44.3: Channel invariant might not hold on action entry (#29)"} (forall i: int :: 
-    (1 <= i) && (i < (R[Net#d] + C[Net#d])) ==> (M[Net#d][i] > M[Net#d][i - 1])
-  );
-  assert {:msg "  45.3: Channel invariant might not hold on action entry (#30)"} (forall i: int :: 
-    (1 <= i) && (i < (R[Net#e] + C[Net#e])) ==> (M[Net#e][i] > M[Net#e][i - 1])
-  );
-  assert {:msg "  47.3: Channel invariant might not hold on action entry (#31)"} C[Net#f] == 1;
-  assert {:msg "  48.3: Channel invariant might not hold on action entry (#32)"} C[Net#g] == R[Net#e];
-  assert {:msg "  49.3: Channel invariant might not hold on action entry (#33)"} R[Net#e] == M[Net#f][R[Net#f]];
-  assert {:msg "  50.3: Channel invariant might not hold on action entry (#34)"} R[Net#d] <= R[Net#e];
-  assert {:msg "  51.3: Channel invariant might not hold on action entry (#35)"} (0 < R[Net#d]) && (0 < R[Net#e]) ==> (M[Net#d][R[Net#d] - 1] <= M[Net#e][R[Net#e] - 1]);
-  assert {:msg "  52.3: Channel invariant might not hold on action entry (#36)"} (forall i: int :: 
+  assert {:msg "  40.3: Channel invariant might not hold on action entry (#25)"} (R[Net#a] + C[Net#a]) <= 3;
+  assert {:msg "  47.3: Channel invariant might not hold on action entry (#26)"} C[Net#f] == 1;
+  assert {:msg "  48.3: Channel invariant might not hold on action entry (#27)"} C[Net#g] == R[Net#e];
+  assert {:msg "  49.3: Channel invariant might not hold on action entry (#28)"} R[Net#e] == M[Net#f][R[Net#f]];
+  assert {:msg "  50.3: Channel invariant might not hold on action entry (#29)"} R[Net#d] <= R[Net#e];
+  assert {:msg "  51.3: Channel invariant might not hold on action entry (#30)"} (0 < R[Net#d]) && (0 < R[Net#e]) ==> (M[Net#d][R[Net#d] - 1] <= M[Net#e][R[Net#e] - 1]);
+  assert {:msg "  52.3: Channel invariant might not hold on action entry (#31)"} (forall i: int :: 
     (0 <= i) && (i < R[Net#e]) ==> (M[Net#g][i] == M[Net#e][i])
   );
 }
@@ -185,9 +185,10 @@ procedure Net#anon$2#Split#anon$1#7()
 {
   var ActionPH#y1: int;
   var ActionPH#y2: int;
+  var ActionPH#y3: int;
   var St#next: State;
   var in#i: int;
-  assume L[Net#a] == (2 * Base#L);
+  assume L[Net#a] == (3 * Base#L);
   assume 0 <= R[Net#a];
   assume 0 <= C[Net#a];
   assume (R[Net#a] + C[Net#a]) <= L[Net#a];
@@ -204,7 +205,7 @@ procedure Net#anon$2#Split#anon$1#7()
   assume 0 <= R[Net#g];
   assume 0 <= C[Net#g];
   assume R[Net#g] == 0;
-  assume (M[Net#a][0] == 0) && (M[Net#a][1] == 1);
+  assume (M[Net#a][0] == 0) && (M[Net#a][1] == 1) && (M[Net#a][2] == 2);
   assume R[Net#a] == (R[Net#b] + C[Net#b]);
   assume R[Net#a] == (R[Net#c] + C[Net#c]);
   assume R[Net#b] == (R[Net#d] + C[Net#d]);
@@ -221,22 +222,7 @@ procedure Net#anon$2#Split#anon$1#7()
   assume (forall idx$: int :: 
     (0 <= idx$) && (idx$ < (R[Net#e] + C[Net#e])) ==> (M[Net#e][idx$] == M[Net#c][idx$])
   );
-  assume (R[Net#a] + C[Net#a]) <= 2;
-  assume (forall i: int :: 
-    (1 <= i) && (i < (R[Net#a] + C[Net#a])) ==> (M[Net#a][i] > M[Net#a][i - 1])
-  );
-  assume (forall i: int :: 
-    (1 <= i) && (i < (R[Net#b] + C[Net#b])) ==> (M[Net#b][i] > M[Net#b][i - 1])
-  );
-  assume (forall i: int :: 
-    (1 <= i) && (i < (R[Net#c] + C[Net#c])) ==> (M[Net#c][i] > M[Net#c][i - 1])
-  );
-  assume (forall i: int :: 
-    (1 <= i) && (i < (R[Net#d] + C[Net#d])) ==> (M[Net#d][i] > M[Net#d][i - 1])
-  );
-  assume (forall i: int :: 
-    (1 <= i) && (i < (R[Net#e] + C[Net#e])) ==> (M[Net#e][i] > M[Net#e][i - 1])
-  );
+  assume (R[Net#a] + C[Net#a]) <= 3;
   assume C[Net#f] == 1;
   assume C[Net#g] == R[Net#e];
   assume R[Net#e] == M[Net#f][R[Net#f]];
@@ -270,45 +256,30 @@ procedure Net#anon$2#Split#anon$1#7()
   assume 0 <= R[Net#g];
   assume 0 <= C[Net#g];
   assume R[Net#g] == 0;
-  assert {:msg "  Action at 8.3 ('anon$1') for actor instance 'spl' might not preserve the channel invariant (#53)"} (M[Net#a][0] == 0) && (M[Net#a][1] == 1);
-  assert {:msg "  Action at 8.3 ('anon$1') for actor instance 'spl' might not preserve the channel invariant (#54)"} R[Net#a] == (R[Net#b] + C[Net#b]);
-  assert {:msg "  Action at 8.3 ('anon$1') for actor instance 'spl' might not preserve the channel invariant (#55)"} R[Net#a] == (R[Net#c] + C[Net#c]);
-  assert {:msg "  Action at 8.3 ('anon$1') for actor instance 'spl' might not preserve the channel invariant (#56)"} R[Net#b] == (R[Net#d] + C[Net#d]);
-  assert {:msg "  Action at 8.3 ('anon$1') for actor instance 'spl' might not preserve the channel invariant (#57)"} R[Net#c] == (R[Net#e] + C[Net#e]);
-  assert {:msg "  Action at 8.3 ('anon$1') for actor instance 'spl' might not preserve the channel invariant (#58)"} (forall idx$: int :: 
+  assert {:msg "  Action at 8.3 ('anon$1') for actor instance 'spl' might not preserve the channel invariant (#48)"} (M[Net#a][0] == 0) && (M[Net#a][1] == 1) && (M[Net#a][2] == 2);
+  assert {:msg "  Action at 8.3 ('anon$1') for actor instance 'spl' might not preserve the channel invariant (#49)"} R[Net#a] == (R[Net#b] + C[Net#b]);
+  assert {:msg "  Action at 8.3 ('anon$1') for actor instance 'spl' might not preserve the channel invariant (#50)"} R[Net#a] == (R[Net#c] + C[Net#c]);
+  assert {:msg "  Action at 8.3 ('anon$1') for actor instance 'spl' might not preserve the channel invariant (#51)"} R[Net#b] == (R[Net#d] + C[Net#d]);
+  assert {:msg "  Action at 8.3 ('anon$1') for actor instance 'spl' might not preserve the channel invariant (#52)"} R[Net#c] == (R[Net#e] + C[Net#e]);
+  assert {:msg "  Action at 8.3 ('anon$1') for actor instance 'spl' might not preserve the channel invariant (#53)"} (forall idx$: int :: 
     (0 <= idx$) && (idx$ < (R[Net#b] + C[Net#b])) ==> (M[Net#b][idx$] == M[Net#a][idx$])
   );
-  assert {:msg "  Action at 8.3 ('anon$1') for actor instance 'spl' might not preserve the channel invariant (#59)"} (forall idx$: int :: 
+  assert {:msg "  Action at 8.3 ('anon$1') for actor instance 'spl' might not preserve the channel invariant (#54)"} (forall idx$: int :: 
     (0 <= idx$) && (idx$ < (R[Net#c] + C[Net#c])) ==> (M[Net#c][idx$] == M[Net#a][idx$])
   );
-  assert {:msg "  Action at 8.3 ('anon$1') for actor instance 'spl' might not preserve the channel invariant (#60)"} (forall idx$: int :: 
+  assert {:msg "  Action at 8.3 ('anon$1') for actor instance 'spl' might not preserve the channel invariant (#55)"} (forall idx$: int :: 
     (0 <= idx$) && (idx$ < (R[Net#d] + C[Net#d])) ==> (M[Net#d][idx$] == M[Net#b][idx$])
   );
-  assert {:msg "  Action at 8.3 ('anon$1') for actor instance 'spl' might not preserve the channel invariant (#61)"} (forall idx$: int :: 
+  assert {:msg "  Action at 8.3 ('anon$1') for actor instance 'spl' might not preserve the channel invariant (#56)"} (forall idx$: int :: 
     (0 <= idx$) && (idx$ < (R[Net#e] + C[Net#e])) ==> (M[Net#e][idx$] == M[Net#c][idx$])
   );
-  assert {:msg "  40.3: Action at 8.3 ('anon$1') for actor instance 'spl' might not preserve the channel invariant (#62)"} (R[Net#a] + C[Net#a]) <= 2;
-  assert {:msg "  41.3: Action at 8.3 ('anon$1') for actor instance 'spl' might not preserve the channel invariant (#63)"} (forall i: int :: 
-    (1 <= i) && (i < (R[Net#a] + C[Net#a])) ==> (M[Net#a][i] > M[Net#a][i - 1])
-  );
-  assert {:msg "  42.3: Action at 8.3 ('anon$1') for actor instance 'spl' might not preserve the channel invariant (#64)"} (forall i: int :: 
-    (1 <= i) && (i < (R[Net#b] + C[Net#b])) ==> (M[Net#b][i] > M[Net#b][i - 1])
-  );
-  assert {:msg "  43.3: Action at 8.3 ('anon$1') for actor instance 'spl' might not preserve the channel invariant (#65)"} (forall i: int :: 
-    (1 <= i) && (i < (R[Net#c] + C[Net#c])) ==> (M[Net#c][i] > M[Net#c][i - 1])
-  );
-  assert {:msg "  44.3: Action at 8.3 ('anon$1') for actor instance 'spl' might not preserve the channel invariant (#66)"} (forall i: int :: 
-    (1 <= i) && (i < (R[Net#d] + C[Net#d])) ==> (M[Net#d][i] > M[Net#d][i - 1])
-  );
-  assert {:msg "  45.3: Action at 8.3 ('anon$1') for actor instance 'spl' might not preserve the channel invariant (#67)"} (forall i: int :: 
-    (1 <= i) && (i < (R[Net#e] + C[Net#e])) ==> (M[Net#e][i] > M[Net#e][i - 1])
-  );
-  assert {:msg "  47.3: Action at 8.3 ('anon$1') for actor instance 'spl' might not preserve the channel invariant (#68)"} C[Net#f] == 1;
-  assert {:msg "  48.3: Action at 8.3 ('anon$1') for actor instance 'spl' might not preserve the channel invariant (#69)"} C[Net#g] == R[Net#e];
-  assert {:msg "  49.3: Action at 8.3 ('anon$1') for actor instance 'spl' might not preserve the channel invariant (#70)"} R[Net#e] == M[Net#f][R[Net#f]];
-  assert {:msg "  50.3: Action at 8.3 ('anon$1') for actor instance 'spl' might not preserve the channel invariant (#71)"} R[Net#d] <= R[Net#e];
-  assert {:msg "  51.3: Action at 8.3 ('anon$1') for actor instance 'spl' might not preserve the channel invariant (#72)"} (0 < R[Net#d]) && (0 < R[Net#e]) ==> (M[Net#d][R[Net#d] - 1] <= M[Net#e][R[Net#e] - 1]);
-  assert {:msg "  52.3: Action at 8.3 ('anon$1') for actor instance 'spl' might not preserve the channel invariant (#73)"} (forall i: int :: 
+  assert {:msg "  40.3: Action at 8.3 ('anon$1') for actor instance 'spl' might not preserve the channel invariant (#57)"} (R[Net#a] + C[Net#a]) <= 3;
+  assert {:msg "  47.3: Action at 8.3 ('anon$1') for actor instance 'spl' might not preserve the channel invariant (#58)"} C[Net#f] == 1;
+  assert {:msg "  48.3: Action at 8.3 ('anon$1') for actor instance 'spl' might not preserve the channel invariant (#59)"} C[Net#g] == R[Net#e];
+  assert {:msg "  49.3: Action at 8.3 ('anon$1') for actor instance 'spl' might not preserve the channel invariant (#60)"} R[Net#e] == M[Net#f][R[Net#f]];
+  assert {:msg "  50.3: Action at 8.3 ('anon$1') for actor instance 'spl' might not preserve the channel invariant (#61)"} R[Net#d] <= R[Net#e];
+  assert {:msg "  51.3: Action at 8.3 ('anon$1') for actor instance 'spl' might not preserve the channel invariant (#62)"} (0 < R[Net#d]) && (0 < R[Net#e]) ==> (M[Net#d][R[Net#d] - 1] <= M[Net#e][R[Net#e] - 1]);
+  assert {:msg "  52.3: Action at 8.3 ('anon$1') for actor instance 'spl' might not preserve the channel invariant (#63)"} (forall i: int :: 
     (0 <= i) && (i < R[Net#e]) ==> (M[Net#g][i] == M[Net#e][i])
   );
 }
@@ -317,9 +288,10 @@ procedure Net#anon$2#Rep#anon$0#8()
 {
   var ActionPH#y1: int;
   var ActionPH#y2: int;
+  var ActionPH#y3: int;
   var St#next: State;
   var in#i: int;
-  assume L[Net#a] == (2 * Base#L);
+  assume L[Net#a] == (3 * Base#L);
   assume 0 <= R[Net#a];
   assume 0 <= C[Net#a];
   assume (R[Net#a] + C[Net#a]) <= L[Net#a];
@@ -336,7 +308,7 @@ procedure Net#anon$2#Rep#anon$0#8()
   assume 0 <= R[Net#g];
   assume 0 <= C[Net#g];
   assume R[Net#g] == 0;
-  assume (M[Net#a][0] == 0) && (M[Net#a][1] == 1);
+  assume (M[Net#a][0] == 0) && (M[Net#a][1] == 1) && (M[Net#a][2] == 2);
   assume R[Net#a] == (R[Net#b] + C[Net#b]);
   assume R[Net#a] == (R[Net#c] + C[Net#c]);
   assume R[Net#b] == (R[Net#d] + C[Net#d]);
@@ -353,22 +325,7 @@ procedure Net#anon$2#Rep#anon$0#8()
   assume (forall idx$: int :: 
     (0 <= idx$) && (idx$ < (R[Net#e] + C[Net#e])) ==> (M[Net#e][idx$] == M[Net#c][idx$])
   );
-  assume (R[Net#a] + C[Net#a]) <= 2;
-  assume (forall i: int :: 
-    (1 <= i) && (i < (R[Net#a] + C[Net#a])) ==> (M[Net#a][i] > M[Net#a][i - 1])
-  );
-  assume (forall i: int :: 
-    (1 <= i) && (i < (R[Net#b] + C[Net#b])) ==> (M[Net#b][i] > M[Net#b][i - 1])
-  );
-  assume (forall i: int :: 
-    (1 <= i) && (i < (R[Net#c] + C[Net#c])) ==> (M[Net#c][i] > M[Net#c][i - 1])
-  );
-  assume (forall i: int :: 
-    (1 <= i) && (i < (R[Net#d] + C[Net#d])) ==> (M[Net#d][i] > M[Net#d][i - 1])
-  );
-  assume (forall i: int :: 
-    (1 <= i) && (i < (R[Net#e] + C[Net#e])) ==> (M[Net#e][i] > M[Net#e][i - 1])
-  );
+  assume (R[Net#a] + C[Net#a]) <= 3;
   assume C[Net#f] == 1;
   assume C[Net#g] == R[Net#e];
   assume R[Net#e] == M[Net#f][R[Net#f]];
@@ -400,45 +357,30 @@ procedure Net#anon$2#Rep#anon$0#8()
   assume 0 <= R[Net#g];
   assume 0 <= C[Net#g];
   assume R[Net#g] == 0;
-  assert {:msg "  Action at 3.3 ('anon$0') for actor instance 'pri' might not preserve the channel invariant (#90)"} (M[Net#a][0] == 0) && (M[Net#a][1] == 1);
-  assert {:msg "  Action at 3.3 ('anon$0') for actor instance 'pri' might not preserve the channel invariant (#91)"} R[Net#a] == (R[Net#b] + C[Net#b]);
-  assert {:msg "  Action at 3.3 ('anon$0') for actor instance 'pri' might not preserve the channel invariant (#92)"} R[Net#a] == (R[Net#c] + C[Net#c]);
-  assert {:msg "  Action at 3.3 ('anon$0') for actor instance 'pri' might not preserve the channel invariant (#93)"} R[Net#b] == (R[Net#d] + C[Net#d]);
-  assert {:msg "  Action at 3.3 ('anon$0') for actor instance 'pri' might not preserve the channel invariant (#94)"} R[Net#c] == (R[Net#e] + C[Net#e]);
-  assert {:msg "  Action at 3.3 ('anon$0') for actor instance 'pri' might not preserve the channel invariant (#95)"} (forall idx$: int :: 
+  assert {:msg "  Action at 3.3 ('anon$0') for actor instance 'pri' might not preserve the channel invariant (#80)"} (M[Net#a][0] == 0) && (M[Net#a][1] == 1) && (M[Net#a][2] == 2);
+  assert {:msg "  Action at 3.3 ('anon$0') for actor instance 'pri' might not preserve the channel invariant (#81)"} R[Net#a] == (R[Net#b] + C[Net#b]);
+  assert {:msg "  Action at 3.3 ('anon$0') for actor instance 'pri' might not preserve the channel invariant (#82)"} R[Net#a] == (R[Net#c] + C[Net#c]);
+  assert {:msg "  Action at 3.3 ('anon$0') for actor instance 'pri' might not preserve the channel invariant (#83)"} R[Net#b] == (R[Net#d] + C[Net#d]);
+  assert {:msg "  Action at 3.3 ('anon$0') for actor instance 'pri' might not preserve the channel invariant (#84)"} R[Net#c] == (R[Net#e] + C[Net#e]);
+  assert {:msg "  Action at 3.3 ('anon$0') for actor instance 'pri' might not preserve the channel invariant (#85)"} (forall idx$: int :: 
     (0 <= idx$) && (idx$ < (R[Net#b] + C[Net#b])) ==> (M[Net#b][idx$] == M[Net#a][idx$])
   );
-  assert {:msg "  Action at 3.3 ('anon$0') for actor instance 'pri' might not preserve the channel invariant (#96)"} (forall idx$: int :: 
+  assert {:msg "  Action at 3.3 ('anon$0') for actor instance 'pri' might not preserve the channel invariant (#86)"} (forall idx$: int :: 
     (0 <= idx$) && (idx$ < (R[Net#c] + C[Net#c])) ==> (M[Net#c][idx$] == M[Net#a][idx$])
   );
-  assert {:msg "  Action at 3.3 ('anon$0') for actor instance 'pri' might not preserve the channel invariant (#97)"} (forall idx$: int :: 
+  assert {:msg "  Action at 3.3 ('anon$0') for actor instance 'pri' might not preserve the channel invariant (#87)"} (forall idx$: int :: 
     (0 <= idx$) && (idx$ < (R[Net#d] + C[Net#d])) ==> (M[Net#d][idx$] == M[Net#b][idx$])
   );
-  assert {:msg "  Action at 3.3 ('anon$0') for actor instance 'pri' might not preserve the channel invariant (#98)"} (forall idx$: int :: 
+  assert {:msg "  Action at 3.3 ('anon$0') for actor instance 'pri' might not preserve the channel invariant (#88)"} (forall idx$: int :: 
     (0 <= idx$) && (idx$ < (R[Net#e] + C[Net#e])) ==> (M[Net#e][idx$] == M[Net#c][idx$])
   );
-  assert {:msg "  40.3: Action at 3.3 ('anon$0') for actor instance 'pri' might not preserve the channel invariant (#99)"} (R[Net#a] + C[Net#a]) <= 2;
-  assert {:msg "  41.3: Action at 3.3 ('anon$0') for actor instance 'pri' might not preserve the channel invariant (#100)"} (forall i: int :: 
-    (1 <= i) && (i < (R[Net#a] + C[Net#a])) ==> (M[Net#a][i] > M[Net#a][i - 1])
-  );
-  assert {:msg "  42.3: Action at 3.3 ('anon$0') for actor instance 'pri' might not preserve the channel invariant (#101)"} (forall i: int :: 
-    (1 <= i) && (i < (R[Net#b] + C[Net#b])) ==> (M[Net#b][i] > M[Net#b][i - 1])
-  );
-  assert {:msg "  43.3: Action at 3.3 ('anon$0') for actor instance 'pri' might not preserve the channel invariant (#102)"} (forall i: int :: 
-    (1 <= i) && (i < (R[Net#c] + C[Net#c])) ==> (M[Net#c][i] > M[Net#c][i - 1])
-  );
-  assert {:msg "  44.3: Action at 3.3 ('anon$0') for actor instance 'pri' might not preserve the channel invariant (#103)"} (forall i: int :: 
-    (1 <= i) && (i < (R[Net#d] + C[Net#d])) ==> (M[Net#d][i] > M[Net#d][i - 1])
-  );
-  assert {:msg "  45.3: Action at 3.3 ('anon$0') for actor instance 'pri' might not preserve the channel invariant (#104)"} (forall i: int :: 
-    (1 <= i) && (i < (R[Net#e] + C[Net#e])) ==> (M[Net#e][i] > M[Net#e][i - 1])
-  );
-  assert {:msg "  47.3: Action at 3.3 ('anon$0') for actor instance 'pri' might not preserve the channel invariant (#105)"} C[Net#f] == 1;
-  assert {:msg "  48.3: Action at 3.3 ('anon$0') for actor instance 'pri' might not preserve the channel invariant (#106)"} C[Net#g] == R[Net#e];
-  assert {:msg "  49.3: Action at 3.3 ('anon$0') for actor instance 'pri' might not preserve the channel invariant (#107)"} R[Net#e] == M[Net#f][R[Net#f]];
-  assert {:msg "  50.3: Action at 3.3 ('anon$0') for actor instance 'pri' might not preserve the channel invariant (#108)"} R[Net#d] <= R[Net#e];
-  assert {:msg "  51.3: Action at 3.3 ('anon$0') for actor instance 'pri' might not preserve the channel invariant (#109)"} (0 < R[Net#d]) && (0 < R[Net#e]) ==> (M[Net#d][R[Net#d] - 1] <= M[Net#e][R[Net#e] - 1]);
-  assert {:msg "  52.3: Action at 3.3 ('anon$0') for actor instance 'pri' might not preserve the channel invariant (#110)"} (forall i: int :: 
+  assert {:msg "  40.3: Action at 3.3 ('anon$0') for actor instance 'pri' might not preserve the channel invariant (#89)"} (R[Net#a] + C[Net#a]) <= 3;
+  assert {:msg "  47.3: Action at 3.3 ('anon$0') for actor instance 'pri' might not preserve the channel invariant (#90)"} C[Net#f] == 1;
+  assert {:msg "  48.3: Action at 3.3 ('anon$0') for actor instance 'pri' might not preserve the channel invariant (#91)"} C[Net#g] == R[Net#e];
+  assert {:msg "  49.3: Action at 3.3 ('anon$0') for actor instance 'pri' might not preserve the channel invariant (#92)"} R[Net#e] == M[Net#f][R[Net#f]];
+  assert {:msg "  50.3: Action at 3.3 ('anon$0') for actor instance 'pri' might not preserve the channel invariant (#93)"} R[Net#d] <= R[Net#e];
+  assert {:msg "  51.3: Action at 3.3 ('anon$0') for actor instance 'pri' might not preserve the channel invariant (#94)"} (0 < R[Net#d]) && (0 < R[Net#e]) ==> (M[Net#d][R[Net#d] - 1] <= M[Net#e][R[Net#e] - 1]);
+  assert {:msg "  52.3: Action at 3.3 ('anon$0') for actor instance 'pri' might not preserve the channel invariant (#95)"} (forall i: int :: 
     (0 <= i) && (i < R[Net#e]) ==> (M[Net#g][i] == M[Net#e][i])
   );
 }
@@ -447,9 +389,10 @@ procedure Net#anon$2#Rep#anon$0#9()
 {
   var ActionPH#y1: int;
   var ActionPH#y2: int;
+  var ActionPH#y3: int;
   var St#next: State;
   var in#i: int;
-  assume L[Net#a] == (2 * Base#L);
+  assume L[Net#a] == (3 * Base#L);
   assume 0 <= R[Net#a];
   assume 0 <= C[Net#a];
   assume (R[Net#a] + C[Net#a]) <= L[Net#a];
@@ -466,7 +409,7 @@ procedure Net#anon$2#Rep#anon$0#9()
   assume 0 <= R[Net#g];
   assume 0 <= C[Net#g];
   assume R[Net#g] == 0;
-  assume (M[Net#a][0] == 0) && (M[Net#a][1] == 1);
+  assume (M[Net#a][0] == 0) && (M[Net#a][1] == 1) && (M[Net#a][2] == 2);
   assume R[Net#a] == (R[Net#b] + C[Net#b]);
   assume R[Net#a] == (R[Net#c] + C[Net#c]);
   assume R[Net#b] == (R[Net#d] + C[Net#d]);
@@ -483,22 +426,7 @@ procedure Net#anon$2#Rep#anon$0#9()
   assume (forall idx$: int :: 
     (0 <= idx$) && (idx$ < (R[Net#e] + C[Net#e])) ==> (M[Net#e][idx$] == M[Net#c][idx$])
   );
-  assume (R[Net#a] + C[Net#a]) <= 2;
-  assume (forall i: int :: 
-    (1 <= i) && (i < (R[Net#a] + C[Net#a])) ==> (M[Net#a][i] > M[Net#a][i - 1])
-  );
-  assume (forall i: int :: 
-    (1 <= i) && (i < (R[Net#b] + C[Net#b])) ==> (M[Net#b][i] > M[Net#b][i - 1])
-  );
-  assume (forall i: int :: 
-    (1 <= i) && (i < (R[Net#c] + C[Net#c])) ==> (M[Net#c][i] > M[Net#c][i - 1])
-  );
-  assume (forall i: int :: 
-    (1 <= i) && (i < (R[Net#d] + C[Net#d])) ==> (M[Net#d][i] > M[Net#d][i - 1])
-  );
-  assume (forall i: int :: 
-    (1 <= i) && (i < (R[Net#e] + C[Net#e])) ==> (M[Net#e][i] > M[Net#e][i - 1])
-  );
+  assume (R[Net#a] + C[Net#a]) <= 3;
   assume C[Net#f] == 1;
   assume C[Net#g] == R[Net#e];
   assume R[Net#e] == M[Net#f][R[Net#f]];
@@ -530,45 +458,30 @@ procedure Net#anon$2#Rep#anon$0#9()
   assume 0 <= R[Net#g];
   assume 0 <= C[Net#g];
   assume R[Net#g] == 0;
-  assert {:msg "  Action at 3.3 ('anon$0') for actor instance 'sec' might not preserve the channel invariant (#127)"} (M[Net#a][0] == 0) && (M[Net#a][1] == 1);
-  assert {:msg "  Action at 3.3 ('anon$0') for actor instance 'sec' might not preserve the channel invariant (#128)"} R[Net#a] == (R[Net#b] + C[Net#b]);
-  assert {:msg "  Action at 3.3 ('anon$0') for actor instance 'sec' might not preserve the channel invariant (#129)"} R[Net#a] == (R[Net#c] + C[Net#c]);
-  assert {:msg "  Action at 3.3 ('anon$0') for actor instance 'sec' might not preserve the channel invariant (#130)"} R[Net#b] == (R[Net#d] + C[Net#d]);
-  assert {:msg "  Action at 3.3 ('anon$0') for actor instance 'sec' might not preserve the channel invariant (#131)"} R[Net#c] == (R[Net#e] + C[Net#e]);
-  assert {:msg "  Action at 3.3 ('anon$0') for actor instance 'sec' might not preserve the channel invariant (#132)"} (forall idx$: int :: 
+  assert {:msg "  Action at 3.3 ('anon$0') for actor instance 'sec' might not preserve the channel invariant (#112)"} (M[Net#a][0] == 0) && (M[Net#a][1] == 1) && (M[Net#a][2] == 2);
+  assert {:msg "  Action at 3.3 ('anon$0') for actor instance 'sec' might not preserve the channel invariant (#113)"} R[Net#a] == (R[Net#b] + C[Net#b]);
+  assert {:msg "  Action at 3.3 ('anon$0') for actor instance 'sec' might not preserve the channel invariant (#114)"} R[Net#a] == (R[Net#c] + C[Net#c]);
+  assert {:msg "  Action at 3.3 ('anon$0') for actor instance 'sec' might not preserve the channel invariant (#115)"} R[Net#b] == (R[Net#d] + C[Net#d]);
+  assert {:msg "  Action at 3.3 ('anon$0') for actor instance 'sec' might not preserve the channel invariant (#116)"} R[Net#c] == (R[Net#e] + C[Net#e]);
+  assert {:msg "  Action at 3.3 ('anon$0') for actor instance 'sec' might not preserve the channel invariant (#117)"} (forall idx$: int :: 
     (0 <= idx$) && (idx$ < (R[Net#b] + C[Net#b])) ==> (M[Net#b][idx$] == M[Net#a][idx$])
   );
-  assert {:msg "  Action at 3.3 ('anon$0') for actor instance 'sec' might not preserve the channel invariant (#133)"} (forall idx$: int :: 
+  assert {:msg "  Action at 3.3 ('anon$0') for actor instance 'sec' might not preserve the channel invariant (#118)"} (forall idx$: int :: 
     (0 <= idx$) && (idx$ < (R[Net#c] + C[Net#c])) ==> (M[Net#c][idx$] == M[Net#a][idx$])
   );
-  assert {:msg "  Action at 3.3 ('anon$0') for actor instance 'sec' might not preserve the channel invariant (#134)"} (forall idx$: int :: 
+  assert {:msg "  Action at 3.3 ('anon$0') for actor instance 'sec' might not preserve the channel invariant (#119)"} (forall idx$: int :: 
     (0 <= idx$) && (idx$ < (R[Net#d] + C[Net#d])) ==> (M[Net#d][idx$] == M[Net#b][idx$])
   );
-  assert {:msg "  Action at 3.3 ('anon$0') for actor instance 'sec' might not preserve the channel invariant (#135)"} (forall idx$: int :: 
+  assert {:msg "  Action at 3.3 ('anon$0') for actor instance 'sec' might not preserve the channel invariant (#120)"} (forall idx$: int :: 
     (0 <= idx$) && (idx$ < (R[Net#e] + C[Net#e])) ==> (M[Net#e][idx$] == M[Net#c][idx$])
   );
-  assert {:msg "  40.3: Action at 3.3 ('anon$0') for actor instance 'sec' might not preserve the channel invariant (#136)"} (R[Net#a] + C[Net#a]) <= 2;
-  assert {:msg "  41.3: Action at 3.3 ('anon$0') for actor instance 'sec' might not preserve the channel invariant (#137)"} (forall i: int :: 
-    (1 <= i) && (i < (R[Net#a] + C[Net#a])) ==> (M[Net#a][i] > M[Net#a][i - 1])
-  );
-  assert {:msg "  42.3: Action at 3.3 ('anon$0') for actor instance 'sec' might not preserve the channel invariant (#138)"} (forall i: int :: 
-    (1 <= i) && (i < (R[Net#b] + C[Net#b])) ==> (M[Net#b][i] > M[Net#b][i - 1])
-  );
-  assert {:msg "  43.3: Action at 3.3 ('anon$0') for actor instance 'sec' might not preserve the channel invariant (#139)"} (forall i: int :: 
-    (1 <= i) && (i < (R[Net#c] + C[Net#c])) ==> (M[Net#c][i] > M[Net#c][i - 1])
-  );
-  assert {:msg "  44.3: Action at 3.3 ('anon$0') for actor instance 'sec' might not preserve the channel invariant (#140)"} (forall i: int :: 
-    (1 <= i) && (i < (R[Net#d] + C[Net#d])) ==> (M[Net#d][i] > M[Net#d][i - 1])
-  );
-  assert {:msg "  45.3: Action at 3.3 ('anon$0') for actor instance 'sec' might not preserve the channel invariant (#141)"} (forall i: int :: 
-    (1 <= i) && (i < (R[Net#e] + C[Net#e])) ==> (M[Net#e][i] > M[Net#e][i - 1])
-  );
-  assert {:msg "  47.3: Action at 3.3 ('anon$0') for actor instance 'sec' might not preserve the channel invariant (#142)"} C[Net#f] == 1;
-  assert {:msg "  48.3: Action at 3.3 ('anon$0') for actor instance 'sec' might not preserve the channel invariant (#143)"} C[Net#g] == R[Net#e];
-  assert {:msg "  49.3: Action at 3.3 ('anon$0') for actor instance 'sec' might not preserve the channel invariant (#144)"} R[Net#e] == M[Net#f][R[Net#f]];
-  assert {:msg "  50.3: Action at 3.3 ('anon$0') for actor instance 'sec' might not preserve the channel invariant (#145)"} R[Net#d] <= R[Net#e];
-  assert {:msg "  51.3: Action at 3.3 ('anon$0') for actor instance 'sec' might not preserve the channel invariant (#146)"} (0 < R[Net#d]) && (0 < R[Net#e]) ==> (M[Net#d][R[Net#d] - 1] <= M[Net#e][R[Net#e] - 1]);
-  assert {:msg "  52.3: Action at 3.3 ('anon$0') for actor instance 'sec' might not preserve the channel invariant (#147)"} (forall i: int :: 
+  assert {:msg "  40.3: Action at 3.3 ('anon$0') for actor instance 'sec' might not preserve the channel invariant (#121)"} (R[Net#a] + C[Net#a]) <= 3;
+  assert {:msg "  47.3: Action at 3.3 ('anon$0') for actor instance 'sec' might not preserve the channel invariant (#122)"} C[Net#f] == 1;
+  assert {:msg "  48.3: Action at 3.3 ('anon$0') for actor instance 'sec' might not preserve the channel invariant (#123)"} C[Net#g] == R[Net#e];
+  assert {:msg "  49.3: Action at 3.3 ('anon$0') for actor instance 'sec' might not preserve the channel invariant (#124)"} R[Net#e] == M[Net#f][R[Net#f]];
+  assert {:msg "  50.3: Action at 3.3 ('anon$0') for actor instance 'sec' might not preserve the channel invariant (#125)"} R[Net#d] <= R[Net#e];
+  assert {:msg "  51.3: Action at 3.3 ('anon$0') for actor instance 'sec' might not preserve the channel invariant (#126)"} (0 < R[Net#d]) && (0 < R[Net#e]) ==> (M[Net#d][R[Net#d] - 1] <= M[Net#e][R[Net#e] - 1]);
+  assert {:msg "  52.3: Action at 3.3 ('anon$0') for actor instance 'sec' might not preserve the channel invariant (#127)"} (forall i: int :: 
     (0 <= i) && (i < R[Net#e]) ==> (M[Net#g][i] == M[Net#e][i])
   );
 }
@@ -577,10 +490,11 @@ procedure Net#anon$2#Adjudicator#readoff#10()
 {
   var ActionPH#y1: int;
   var ActionPH#y2: int;
+  var ActionPH#y3: int;
   var St#next: State;
   var x1#i: int;
   var c_in#c: int;
-  assume L[Net#a] == (2 * Base#L);
+  assume L[Net#a] == (3 * Base#L);
   assume 0 <= R[Net#a];
   assume 0 <= C[Net#a];
   assume (R[Net#a] + C[Net#a]) <= L[Net#a];
@@ -597,7 +511,7 @@ procedure Net#anon$2#Adjudicator#readoff#10()
   assume 0 <= R[Net#g];
   assume 0 <= C[Net#g];
   assume R[Net#g] == 0;
-  assume (M[Net#a][0] == 0) && (M[Net#a][1] == 1);
+  assume (M[Net#a][0] == 0) && (M[Net#a][1] == 1) && (M[Net#a][2] == 2);
   assume R[Net#a] == (R[Net#b] + C[Net#b]);
   assume R[Net#a] == (R[Net#c] + C[Net#c]);
   assume R[Net#b] == (R[Net#d] + C[Net#d]);
@@ -614,22 +528,7 @@ procedure Net#anon$2#Adjudicator#readoff#10()
   assume (forall idx$: int :: 
     (0 <= idx$) && (idx$ < (R[Net#e] + C[Net#e])) ==> (M[Net#e][idx$] == M[Net#c][idx$])
   );
-  assume (R[Net#a] + C[Net#a]) <= 2;
-  assume (forall i: int :: 
-    (1 <= i) && (i < (R[Net#a] + C[Net#a])) ==> (M[Net#a][i] > M[Net#a][i - 1])
-  );
-  assume (forall i: int :: 
-    (1 <= i) && (i < (R[Net#b] + C[Net#b])) ==> (M[Net#b][i] > M[Net#b][i - 1])
-  );
-  assume (forall i: int :: 
-    (1 <= i) && (i < (R[Net#c] + C[Net#c])) ==> (M[Net#c][i] > M[Net#c][i - 1])
-  );
-  assume (forall i: int :: 
-    (1 <= i) && (i < (R[Net#d] + C[Net#d])) ==> (M[Net#d][i] > M[Net#d][i - 1])
-  );
-  assume (forall i: int :: 
-    (1 <= i) && (i < (R[Net#e] + C[Net#e])) ==> (M[Net#e][i] > M[Net#e][i - 1])
-  );
+  assume (R[Net#a] + C[Net#a]) <= 3;
   assume C[Net#f] == 1;
   assume C[Net#g] == R[Net#e];
   assume R[Net#e] == M[Net#f][R[Net#f]];
@@ -665,45 +564,30 @@ procedure Net#anon$2#Adjudicator#readoff#10()
   assume 0 <= R[Net#g];
   assume 0 <= C[Net#g];
   assume R[Net#g] == 0;
-  assert {:msg "  Action at 22.3 ('readoff') for actor instance 'adj' might not preserve the channel invariant (#164)"} (M[Net#a][0] == 0) && (M[Net#a][1] == 1);
-  assert {:msg "  Action at 22.3 ('readoff') for actor instance 'adj' might not preserve the channel invariant (#165)"} R[Net#a] == (R[Net#b] + C[Net#b]);
-  assert {:msg "  Action at 22.3 ('readoff') for actor instance 'adj' might not preserve the channel invariant (#166)"} R[Net#a] == (R[Net#c] + C[Net#c]);
-  assert {:msg "  Action at 22.3 ('readoff') for actor instance 'adj' might not preserve the channel invariant (#167)"} R[Net#b] == (R[Net#d] + C[Net#d]);
-  assert {:msg "  Action at 22.3 ('readoff') for actor instance 'adj' might not preserve the channel invariant (#168)"} R[Net#c] == (R[Net#e] + C[Net#e]);
-  assert {:msg "  Action at 22.3 ('readoff') for actor instance 'adj' might not preserve the channel invariant (#169)"} (forall idx$: int :: 
+  assert {:msg "  Action at 22.3 ('readoff') for actor instance 'adj' might not preserve the channel invariant (#144)"} (M[Net#a][0] == 0) && (M[Net#a][1] == 1) && (M[Net#a][2] == 2);
+  assert {:msg "  Action at 22.3 ('readoff') for actor instance 'adj' might not preserve the channel invariant (#145)"} R[Net#a] == (R[Net#b] + C[Net#b]);
+  assert {:msg "  Action at 22.3 ('readoff') for actor instance 'adj' might not preserve the channel invariant (#146)"} R[Net#a] == (R[Net#c] + C[Net#c]);
+  assert {:msg "  Action at 22.3 ('readoff') for actor instance 'adj' might not preserve the channel invariant (#147)"} R[Net#b] == (R[Net#d] + C[Net#d]);
+  assert {:msg "  Action at 22.3 ('readoff') for actor instance 'adj' might not preserve the channel invariant (#148)"} R[Net#c] == (R[Net#e] + C[Net#e]);
+  assert {:msg "  Action at 22.3 ('readoff') for actor instance 'adj' might not preserve the channel invariant (#149)"} (forall idx$: int :: 
     (0 <= idx$) && (idx$ < (R[Net#b] + C[Net#b])) ==> (M[Net#b][idx$] == M[Net#a][idx$])
   );
-  assert {:msg "  Action at 22.3 ('readoff') for actor instance 'adj' might not preserve the channel invariant (#170)"} (forall idx$: int :: 
+  assert {:msg "  Action at 22.3 ('readoff') for actor instance 'adj' might not preserve the channel invariant (#150)"} (forall idx$: int :: 
     (0 <= idx$) && (idx$ < (R[Net#c] + C[Net#c])) ==> (M[Net#c][idx$] == M[Net#a][idx$])
   );
-  assert {:msg "  Action at 22.3 ('readoff') for actor instance 'adj' might not preserve the channel invariant (#171)"} (forall idx$: int :: 
+  assert {:msg "  Action at 22.3 ('readoff') for actor instance 'adj' might not preserve the channel invariant (#151)"} (forall idx$: int :: 
     (0 <= idx$) && (idx$ < (R[Net#d] + C[Net#d])) ==> (M[Net#d][idx$] == M[Net#b][idx$])
   );
-  assert {:msg "  Action at 22.3 ('readoff') for actor instance 'adj' might not preserve the channel invariant (#172)"} (forall idx$: int :: 
+  assert {:msg "  Action at 22.3 ('readoff') for actor instance 'adj' might not preserve the channel invariant (#152)"} (forall idx$: int :: 
     (0 <= idx$) && (idx$ < (R[Net#e] + C[Net#e])) ==> (M[Net#e][idx$] == M[Net#c][idx$])
   );
-  assert {:msg "  40.3: Action at 22.3 ('readoff') for actor instance 'adj' might not preserve the channel invariant (#173)"} (R[Net#a] + C[Net#a]) <= 2;
-  assert {:msg "  41.3: Action at 22.3 ('readoff') for actor instance 'adj' might not preserve the channel invariant (#174)"} (forall i: int :: 
-    (1 <= i) && (i < (R[Net#a] + C[Net#a])) ==> (M[Net#a][i] > M[Net#a][i - 1])
-  );
-  assert {:msg "  42.3: Action at 22.3 ('readoff') for actor instance 'adj' might not preserve the channel invariant (#175)"} (forall i: int :: 
-    (1 <= i) && (i < (R[Net#b] + C[Net#b])) ==> (M[Net#b][i] > M[Net#b][i - 1])
-  );
-  assert {:msg "  43.3: Action at 22.3 ('readoff') for actor instance 'adj' might not preserve the channel invariant (#176)"} (forall i: int :: 
-    (1 <= i) && (i < (R[Net#c] + C[Net#c])) ==> (M[Net#c][i] > M[Net#c][i - 1])
-  );
-  assert {:msg "  44.3: Action at 22.3 ('readoff') for actor instance 'adj' might not preserve the channel invariant (#177)"} (forall i: int :: 
-    (1 <= i) && (i < (R[Net#d] + C[Net#d])) ==> (M[Net#d][i] > M[Net#d][i - 1])
-  );
-  assert {:msg "  45.3: Action at 22.3 ('readoff') for actor instance 'adj' might not preserve the channel invariant (#178)"} (forall i: int :: 
-    (1 <= i) && (i < (R[Net#e] + C[Net#e])) ==> (M[Net#e][i] > M[Net#e][i - 1])
-  );
-  assert {:msg "  47.3: Action at 22.3 ('readoff') for actor instance 'adj' might not preserve the channel invariant (#179)"} C[Net#f] == 1;
-  assert {:msg "  48.3: Action at 22.3 ('readoff') for actor instance 'adj' might not preserve the channel invariant (#180)"} C[Net#g] == R[Net#e];
-  assert {:msg "  49.3: Action at 22.3 ('readoff') for actor instance 'adj' might not preserve the channel invariant (#181)"} R[Net#e] == M[Net#f][R[Net#f]];
-  assert {:msg "  50.3: Action at 22.3 ('readoff') for actor instance 'adj' might not preserve the channel invariant (#182)"} R[Net#d] <= R[Net#e];
-  assert {:msg "  51.3: Action at 22.3 ('readoff') for actor instance 'adj' might not preserve the channel invariant (#183)"} (0 < R[Net#d]) && (0 < R[Net#e]) ==> (M[Net#d][R[Net#d] - 1] <= M[Net#e][R[Net#e] - 1]);
-  assert {:msg "  52.3: Action at 22.3 ('readoff') for actor instance 'adj' might not preserve the channel invariant (#184)"} (forall i: int :: 
+  assert {:msg "  40.3: Action at 22.3 ('readoff') for actor instance 'adj' might not preserve the channel invariant (#153)"} (R[Net#a] + C[Net#a]) <= 3;
+  assert {:msg "  47.3: Action at 22.3 ('readoff') for actor instance 'adj' might not preserve the channel invariant (#154)"} C[Net#f] == 1;
+  assert {:msg "  48.3: Action at 22.3 ('readoff') for actor instance 'adj' might not preserve the channel invariant (#155)"} C[Net#g] == R[Net#e];
+  assert {:msg "  49.3: Action at 22.3 ('readoff') for actor instance 'adj' might not preserve the channel invariant (#156)"} R[Net#e] == M[Net#f][R[Net#f]];
+  assert {:msg "  50.3: Action at 22.3 ('readoff') for actor instance 'adj' might not preserve the channel invariant (#157)"} R[Net#d] <= R[Net#e];
+  assert {:msg "  51.3: Action at 22.3 ('readoff') for actor instance 'adj' might not preserve the channel invariant (#158)"} (0 < R[Net#d]) && (0 < R[Net#e]) ==> (M[Net#d][R[Net#d] - 1] <= M[Net#e][R[Net#e] - 1]);
+  assert {:msg "  52.3: Action at 22.3 ('readoff') for actor instance 'adj' might not preserve the channel invariant (#159)"} (forall i: int :: 
     (0 <= i) && (i < R[Net#e]) ==> (M[Net#g][i] == M[Net#e][i])
   );
 }
@@ -712,11 +596,12 @@ procedure Net#anon$2#Adjudicator#normal#11()
 {
   var ActionPH#y1: int;
   var ActionPH#y2: int;
+  var ActionPH#y3: int;
   var St#next: State;
   var x1#i: int;
   var x2#j: int;
   var c_in#c: int;
-  assume L[Net#a] == (2 * Base#L);
+  assume L[Net#a] == (3 * Base#L);
   assume 0 <= R[Net#a];
   assume 0 <= C[Net#a];
   assume (R[Net#a] + C[Net#a]) <= L[Net#a];
@@ -733,7 +618,7 @@ procedure Net#anon$2#Adjudicator#normal#11()
   assume 0 <= R[Net#g];
   assume 0 <= C[Net#g];
   assume R[Net#g] == 0;
-  assume (M[Net#a][0] == 0) && (M[Net#a][1] == 1);
+  assume (M[Net#a][0] == 0) && (M[Net#a][1] == 1) && (M[Net#a][2] == 2);
   assume R[Net#a] == (R[Net#b] + C[Net#b]);
   assume R[Net#a] == (R[Net#c] + C[Net#c]);
   assume R[Net#b] == (R[Net#d] + C[Net#d]);
@@ -750,22 +635,7 @@ procedure Net#anon$2#Adjudicator#normal#11()
   assume (forall idx$: int :: 
     (0 <= idx$) && (idx$ < (R[Net#e] + C[Net#e])) ==> (M[Net#e][idx$] == M[Net#c][idx$])
   );
-  assume (R[Net#a] + C[Net#a]) <= 2;
-  assume (forall i: int :: 
-    (1 <= i) && (i < (R[Net#a] + C[Net#a])) ==> (M[Net#a][i] > M[Net#a][i - 1])
-  );
-  assume (forall i: int :: 
-    (1 <= i) && (i < (R[Net#b] + C[Net#b])) ==> (M[Net#b][i] > M[Net#b][i - 1])
-  );
-  assume (forall i: int :: 
-    (1 <= i) && (i < (R[Net#c] + C[Net#c])) ==> (M[Net#c][i] > M[Net#c][i - 1])
-  );
-  assume (forall i: int :: 
-    (1 <= i) && (i < (R[Net#d] + C[Net#d])) ==> (M[Net#d][i] > M[Net#d][i - 1])
-  );
-  assume (forall i: int :: 
-    (1 <= i) && (i < (R[Net#e] + C[Net#e])) ==> (M[Net#e][i] > M[Net#e][i - 1])
-  );
+  assume (R[Net#a] + C[Net#a]) <= 3;
   assume C[Net#f] == 1;
   assume C[Net#g] == R[Net#e];
   assume R[Net#e] == M[Net#f][R[Net#f]];
@@ -806,45 +676,30 @@ procedure Net#anon$2#Adjudicator#normal#11()
   assume 0 <= R[Net#g];
   assume 0 <= C[Net#g];
   assume R[Net#g] == 0;
-  assert {:msg "  Action at 14.3 ('normal') for actor instance 'adj' might not preserve the channel invariant (#201)"} (M[Net#a][0] == 0) && (M[Net#a][1] == 1);
-  assert {:msg "  Action at 14.3 ('normal') for actor instance 'adj' might not preserve the channel invariant (#202)"} R[Net#a] == (R[Net#b] + C[Net#b]);
-  assert {:msg "  Action at 14.3 ('normal') for actor instance 'adj' might not preserve the channel invariant (#203)"} R[Net#a] == (R[Net#c] + C[Net#c]);
-  assert {:msg "  Action at 14.3 ('normal') for actor instance 'adj' might not preserve the channel invariant (#204)"} R[Net#b] == (R[Net#d] + C[Net#d]);
-  assert {:msg "  Action at 14.3 ('normal') for actor instance 'adj' might not preserve the channel invariant (#205)"} R[Net#c] == (R[Net#e] + C[Net#e]);
-  assert {:msg "  Action at 14.3 ('normal') for actor instance 'adj' might not preserve the channel invariant (#206)"} (forall idx$: int :: 
+  assert {:msg "  Action at 14.3 ('normal') for actor instance 'adj' might not preserve the channel invariant (#176)"} (M[Net#a][0] == 0) && (M[Net#a][1] == 1) && (M[Net#a][2] == 2);
+  assert {:msg "  Action at 14.3 ('normal') for actor instance 'adj' might not preserve the channel invariant (#177)"} R[Net#a] == (R[Net#b] + C[Net#b]);
+  assert {:msg "  Action at 14.3 ('normal') for actor instance 'adj' might not preserve the channel invariant (#178)"} R[Net#a] == (R[Net#c] + C[Net#c]);
+  assert {:msg "  Action at 14.3 ('normal') for actor instance 'adj' might not preserve the channel invariant (#179)"} R[Net#b] == (R[Net#d] + C[Net#d]);
+  assert {:msg "  Action at 14.3 ('normal') for actor instance 'adj' might not preserve the channel invariant (#180)"} R[Net#c] == (R[Net#e] + C[Net#e]);
+  assert {:msg "  Action at 14.3 ('normal') for actor instance 'adj' might not preserve the channel invariant (#181)"} (forall idx$: int :: 
     (0 <= idx$) && (idx$ < (R[Net#b] + C[Net#b])) ==> (M[Net#b][idx$] == M[Net#a][idx$])
   );
-  assert {:msg "  Action at 14.3 ('normal') for actor instance 'adj' might not preserve the channel invariant (#207)"} (forall idx$: int :: 
+  assert {:msg "  Action at 14.3 ('normal') for actor instance 'adj' might not preserve the channel invariant (#182)"} (forall idx$: int :: 
     (0 <= idx$) && (idx$ < (R[Net#c] + C[Net#c])) ==> (M[Net#c][idx$] == M[Net#a][idx$])
   );
-  assert {:msg "  Action at 14.3 ('normal') for actor instance 'adj' might not preserve the channel invariant (#208)"} (forall idx$: int :: 
+  assert {:msg "  Action at 14.3 ('normal') for actor instance 'adj' might not preserve the channel invariant (#183)"} (forall idx$: int :: 
     (0 <= idx$) && (idx$ < (R[Net#d] + C[Net#d])) ==> (M[Net#d][idx$] == M[Net#b][idx$])
   );
-  assert {:msg "  Action at 14.3 ('normal') for actor instance 'adj' might not preserve the channel invariant (#209)"} (forall idx$: int :: 
+  assert {:msg "  Action at 14.3 ('normal') for actor instance 'adj' might not preserve the channel invariant (#184)"} (forall idx$: int :: 
     (0 <= idx$) && (idx$ < (R[Net#e] + C[Net#e])) ==> (M[Net#e][idx$] == M[Net#c][idx$])
   );
-  assert {:msg "  40.3: Action at 14.3 ('normal') for actor instance 'adj' might not preserve the channel invariant (#210)"} (R[Net#a] + C[Net#a]) <= 2;
-  assert {:msg "  41.3: Action at 14.3 ('normal') for actor instance 'adj' might not preserve the channel invariant (#211)"} (forall i: int :: 
-    (1 <= i) && (i < (R[Net#a] + C[Net#a])) ==> (M[Net#a][i] > M[Net#a][i - 1])
-  );
-  assert {:msg "  42.3: Action at 14.3 ('normal') for actor instance 'adj' might not preserve the channel invariant (#212)"} (forall i: int :: 
-    (1 <= i) && (i < (R[Net#b] + C[Net#b])) ==> (M[Net#b][i] > M[Net#b][i - 1])
-  );
-  assert {:msg "  43.3: Action at 14.3 ('normal') for actor instance 'adj' might not preserve the channel invariant (#213)"} (forall i: int :: 
-    (1 <= i) && (i < (R[Net#c] + C[Net#c])) ==> (M[Net#c][i] > M[Net#c][i - 1])
-  );
-  assert {:msg "  44.3: Action at 14.3 ('normal') for actor instance 'adj' might not preserve the channel invariant (#214)"} (forall i: int :: 
-    (1 <= i) && (i < (R[Net#d] + C[Net#d])) ==> (M[Net#d][i] > M[Net#d][i - 1])
-  );
-  assert {:msg "  45.3: Action at 14.3 ('normal') for actor instance 'adj' might not preserve the channel invariant (#215)"} (forall i: int :: 
-    (1 <= i) && (i < (R[Net#e] + C[Net#e])) ==> (M[Net#e][i] > M[Net#e][i - 1])
-  );
-  assert {:msg "  47.3: Action at 14.3 ('normal') for actor instance 'adj' might not preserve the channel invariant (#216)"} C[Net#f] == 1;
-  assert {:msg "  48.3: Action at 14.3 ('normal') for actor instance 'adj' might not preserve the channel invariant (#217)"} C[Net#g] == R[Net#e];
-  assert {:msg "  49.3: Action at 14.3 ('normal') for actor instance 'adj' might not preserve the channel invariant (#218)"} R[Net#e] == M[Net#f][R[Net#f]];
-  assert {:msg "  50.3: Action at 14.3 ('normal') for actor instance 'adj' might not preserve the channel invariant (#219)"} R[Net#d] <= R[Net#e];
-  assert {:msg "  51.3: Action at 14.3 ('normal') for actor instance 'adj' might not preserve the channel invariant (#220)"} (0 < R[Net#d]) && (0 < R[Net#e]) ==> (M[Net#d][R[Net#d] - 1] <= M[Net#e][R[Net#e] - 1]);
-  assert {:msg "  52.3: Action at 14.3 ('normal') for actor instance 'adj' might not preserve the channel invariant (#221)"} (forall i: int :: 
+  assert {:msg "  40.3: Action at 14.3 ('normal') for actor instance 'adj' might not preserve the channel invariant (#185)"} (R[Net#a] + C[Net#a]) <= 3;
+  assert {:msg "  47.3: Action at 14.3 ('normal') for actor instance 'adj' might not preserve the channel invariant (#186)"} C[Net#f] == 1;
+  assert {:msg "  48.3: Action at 14.3 ('normal') for actor instance 'adj' might not preserve the channel invariant (#187)"} C[Net#g] == R[Net#e];
+  assert {:msg "  49.3: Action at 14.3 ('normal') for actor instance 'adj' might not preserve the channel invariant (#188)"} R[Net#e] == M[Net#f][R[Net#f]];
+  assert {:msg "  50.3: Action at 14.3 ('normal') for actor instance 'adj' might not preserve the channel invariant (#189)"} R[Net#d] <= R[Net#e];
+  assert {:msg "  51.3: Action at 14.3 ('normal') for actor instance 'adj' might not preserve the channel invariant (#190)"} (0 < R[Net#d]) && (0 < R[Net#e]) ==> (M[Net#d][R[Net#d] - 1] <= M[Net#e][R[Net#e] - 1]);
+  assert {:msg "  52.3: Action at 14.3 ('normal') for actor instance 'adj' might not preserve the channel invariant (#191)"} (forall i: int :: 
     (0 <= i) && (i < R[Net#e]) ==> (M[Net#g][i] == M[Net#e][i])
   );
 }
@@ -853,10 +708,11 @@ procedure Net#anon$2#Adjudicator#timeout#12()
 {
   var ActionPH#y1: int;
   var ActionPH#y2: int;
+  var ActionPH#y3: int;
   var St#next: State;
   var x2#j: int;
   var c_in#c: int;
-  assume L[Net#a] == (2 * Base#L);
+  assume L[Net#a] == (3 * Base#L);
   assume 0 <= R[Net#a];
   assume 0 <= C[Net#a];
   assume (R[Net#a] + C[Net#a]) <= L[Net#a];
@@ -873,7 +729,7 @@ procedure Net#anon$2#Adjudicator#timeout#12()
   assume 0 <= R[Net#g];
   assume 0 <= C[Net#g];
   assume R[Net#g] == 0;
-  assume (M[Net#a][0] == 0) && (M[Net#a][1] == 1);
+  assume (M[Net#a][0] == 0) && (M[Net#a][1] == 1) && (M[Net#a][2] == 2);
   assume R[Net#a] == (R[Net#b] + C[Net#b]);
   assume R[Net#a] == (R[Net#c] + C[Net#c]);
   assume R[Net#b] == (R[Net#d] + C[Net#d]);
@@ -890,22 +746,7 @@ procedure Net#anon$2#Adjudicator#timeout#12()
   assume (forall idx$: int :: 
     (0 <= idx$) && (idx$ < (R[Net#e] + C[Net#e])) ==> (M[Net#e][idx$] == M[Net#c][idx$])
   );
-  assume (R[Net#a] + C[Net#a]) <= 2;
-  assume (forall i: int :: 
-    (1 <= i) && (i < (R[Net#a] + C[Net#a])) ==> (M[Net#a][i] > M[Net#a][i - 1])
-  );
-  assume (forall i: int :: 
-    (1 <= i) && (i < (R[Net#b] + C[Net#b])) ==> (M[Net#b][i] > M[Net#b][i - 1])
-  );
-  assume (forall i: int :: 
-    (1 <= i) && (i < (R[Net#c] + C[Net#c])) ==> (M[Net#c][i] > M[Net#c][i - 1])
-  );
-  assume (forall i: int :: 
-    (1 <= i) && (i < (R[Net#d] + C[Net#d])) ==> (M[Net#d][i] > M[Net#d][i - 1])
-  );
-  assume (forall i: int :: 
-    (1 <= i) && (i < (R[Net#e] + C[Net#e])) ==> (M[Net#e][i] > M[Net#e][i - 1])
-  );
+  assume (R[Net#a] + C[Net#a]) <= 3;
   assume C[Net#f] == 1;
   assume C[Net#g] == R[Net#e];
   assume R[Net#e] == M[Net#f][R[Net#f]];
@@ -942,45 +783,30 @@ procedure Net#anon$2#Adjudicator#timeout#12()
   assume 0 <= R[Net#g];
   assume 0 <= C[Net#g];
   assume R[Net#g] == 0;
-  assert {:msg "  Action at 18.3 ('timeout') for actor instance 'adj' might not preserve the channel invariant (#238)"} (M[Net#a][0] == 0) && (M[Net#a][1] == 1);
-  assert {:msg "  Action at 18.3 ('timeout') for actor instance 'adj' might not preserve the channel invariant (#239)"} R[Net#a] == (R[Net#b] + C[Net#b]);
-  assert {:msg "  Action at 18.3 ('timeout') for actor instance 'adj' might not preserve the channel invariant (#240)"} R[Net#a] == (R[Net#c] + C[Net#c]);
-  assert {:msg "  Action at 18.3 ('timeout') for actor instance 'adj' might not preserve the channel invariant (#241)"} R[Net#b] == (R[Net#d] + C[Net#d]);
-  assert {:msg "  Action at 18.3 ('timeout') for actor instance 'adj' might not preserve the channel invariant (#242)"} R[Net#c] == (R[Net#e] + C[Net#e]);
-  assert {:msg "  Action at 18.3 ('timeout') for actor instance 'adj' might not preserve the channel invariant (#243)"} (forall idx$: int :: 
+  assert {:msg "  Action at 18.3 ('timeout') for actor instance 'adj' might not preserve the channel invariant (#208)"} (M[Net#a][0] == 0) && (M[Net#a][1] == 1) && (M[Net#a][2] == 2);
+  assert {:msg "  Action at 18.3 ('timeout') for actor instance 'adj' might not preserve the channel invariant (#209)"} R[Net#a] == (R[Net#b] + C[Net#b]);
+  assert {:msg "  Action at 18.3 ('timeout') for actor instance 'adj' might not preserve the channel invariant (#210)"} R[Net#a] == (R[Net#c] + C[Net#c]);
+  assert {:msg "  Action at 18.3 ('timeout') for actor instance 'adj' might not preserve the channel invariant (#211)"} R[Net#b] == (R[Net#d] + C[Net#d]);
+  assert {:msg "  Action at 18.3 ('timeout') for actor instance 'adj' might not preserve the channel invariant (#212)"} R[Net#c] == (R[Net#e] + C[Net#e]);
+  assert {:msg "  Action at 18.3 ('timeout') for actor instance 'adj' might not preserve the channel invariant (#213)"} (forall idx$: int :: 
     (0 <= idx$) && (idx$ < (R[Net#b] + C[Net#b])) ==> (M[Net#b][idx$] == M[Net#a][idx$])
   );
-  assert {:msg "  Action at 18.3 ('timeout') for actor instance 'adj' might not preserve the channel invariant (#244)"} (forall idx$: int :: 
+  assert {:msg "  Action at 18.3 ('timeout') for actor instance 'adj' might not preserve the channel invariant (#214)"} (forall idx$: int :: 
     (0 <= idx$) && (idx$ < (R[Net#c] + C[Net#c])) ==> (M[Net#c][idx$] == M[Net#a][idx$])
   );
-  assert {:msg "  Action at 18.3 ('timeout') for actor instance 'adj' might not preserve the channel invariant (#245)"} (forall idx$: int :: 
+  assert {:msg "  Action at 18.3 ('timeout') for actor instance 'adj' might not preserve the channel invariant (#215)"} (forall idx$: int :: 
     (0 <= idx$) && (idx$ < (R[Net#d] + C[Net#d])) ==> (M[Net#d][idx$] == M[Net#b][idx$])
   );
-  assert {:msg "  Action at 18.3 ('timeout') for actor instance 'adj' might not preserve the channel invariant (#246)"} (forall idx$: int :: 
+  assert {:msg "  Action at 18.3 ('timeout') for actor instance 'adj' might not preserve the channel invariant (#216)"} (forall idx$: int :: 
     (0 <= idx$) && (idx$ < (R[Net#e] + C[Net#e])) ==> (M[Net#e][idx$] == M[Net#c][idx$])
   );
-  assert {:msg "  40.3: Action at 18.3 ('timeout') for actor instance 'adj' might not preserve the channel invariant (#247)"} (R[Net#a] + C[Net#a]) <= 2;
-  assert {:msg "  41.3: Action at 18.3 ('timeout') for actor instance 'adj' might not preserve the channel invariant (#248)"} (forall i: int :: 
-    (1 <= i) && (i < (R[Net#a] + C[Net#a])) ==> (M[Net#a][i] > M[Net#a][i - 1])
-  );
-  assert {:msg "  42.3: Action at 18.3 ('timeout') for actor instance 'adj' might not preserve the channel invariant (#249)"} (forall i: int :: 
-    (1 <= i) && (i < (R[Net#b] + C[Net#b])) ==> (M[Net#b][i] > M[Net#b][i - 1])
-  );
-  assert {:msg "  43.3: Action at 18.3 ('timeout') for actor instance 'adj' might not preserve the channel invariant (#250)"} (forall i: int :: 
-    (1 <= i) && (i < (R[Net#c] + C[Net#c])) ==> (M[Net#c][i] > M[Net#c][i - 1])
-  );
-  assert {:msg "  44.3: Action at 18.3 ('timeout') for actor instance 'adj' might not preserve the channel invariant (#251)"} (forall i: int :: 
-    (1 <= i) && (i < (R[Net#d] + C[Net#d])) ==> (M[Net#d][i] > M[Net#d][i - 1])
-  );
-  assert {:msg "  45.3: Action at 18.3 ('timeout') for actor instance 'adj' might not preserve the channel invariant (#252)"} (forall i: int :: 
-    (1 <= i) && (i < (R[Net#e] + C[Net#e])) ==> (M[Net#e][i] > M[Net#e][i - 1])
-  );
-  assert {:msg "  47.3: Action at 18.3 ('timeout') for actor instance 'adj' might not preserve the channel invariant (#253)"} C[Net#f] == 1;
-  assert {:msg "  48.3: Action at 18.3 ('timeout') for actor instance 'adj' might not preserve the channel invariant (#254)"} C[Net#g] == R[Net#e];
-  assert {:msg "  49.3: Action at 18.3 ('timeout') for actor instance 'adj' might not preserve the channel invariant (#255)"} R[Net#e] == M[Net#f][R[Net#f]];
-  assert {:msg "  50.3: Action at 18.3 ('timeout') for actor instance 'adj' might not preserve the channel invariant (#256)"} R[Net#d] <= R[Net#e];
-  assert {:msg "  51.3: Action at 18.3 ('timeout') for actor instance 'adj' might not preserve the channel invariant (#257)"} (0 < R[Net#d]) && (0 < R[Net#e]) ==> (M[Net#d][R[Net#d] - 1] <= M[Net#e][R[Net#e] - 1]);
-  assert {:msg "  52.3: Action at 18.3 ('timeout') for actor instance 'adj' might not preserve the channel invariant (#258)"} (forall i: int :: 
+  assert {:msg "  40.3: Action at 18.3 ('timeout') for actor instance 'adj' might not preserve the channel invariant (#217)"} (R[Net#a] + C[Net#a]) <= 3;
+  assert {:msg "  47.3: Action at 18.3 ('timeout') for actor instance 'adj' might not preserve the channel invariant (#218)"} C[Net#f] == 1;
+  assert {:msg "  48.3: Action at 18.3 ('timeout') for actor instance 'adj' might not preserve the channel invariant (#219)"} C[Net#g] == R[Net#e];
+  assert {:msg "  49.3: Action at 18.3 ('timeout') for actor instance 'adj' might not preserve the channel invariant (#220)"} R[Net#e] == M[Net#f][R[Net#f]];
+  assert {:msg "  50.3: Action at 18.3 ('timeout') for actor instance 'adj' might not preserve the channel invariant (#221)"} R[Net#d] <= R[Net#e];
+  assert {:msg "  51.3: Action at 18.3 ('timeout') for actor instance 'adj' might not preserve the channel invariant (#222)"} (0 < R[Net#d]) && (0 < R[Net#e]) ==> (M[Net#d][R[Net#d] - 1] <= M[Net#e][R[Net#e] - 1]);
+  assert {:msg "  52.3: Action at 18.3 ('timeout') for actor instance 'adj' might not preserve the channel invariant (#223)"} (forall i: int :: 
     (0 <= i) && (i < R[Net#e]) ==> (M[Net#g][i] == M[Net#e][i])
   );
 }
@@ -989,7 +815,8 @@ procedure Net#anon$2#exit#13()
 {
   var ActionPH#y1: int;
   var ActionPH#y2: int;
-  assume L[Net#a] == (2 * Base#L);
+  var ActionPH#y3: int;
+  assume L[Net#a] == (3 * Base#L);
   assume 0 <= R[Net#a];
   assume 0 <= C[Net#a];
   assume (R[Net#a] + C[Net#a]) <= L[Net#a];
@@ -1006,7 +833,7 @@ procedure Net#anon$2#exit#13()
   assume 0 <= R[Net#g];
   assume 0 <= C[Net#g];
   assume R[Net#g] == 0;
-  assume (M[Net#a][0] == 0) && (M[Net#a][1] == 1);
+  assume (M[Net#a][0] == 0) && (M[Net#a][1] == 1) && (M[Net#a][2] == 2);
   assume R[Net#a] == (R[Net#b] + C[Net#b]);
   assume R[Net#a] == (R[Net#c] + C[Net#c]);
   assume R[Net#b] == (R[Net#d] + C[Net#d]);
@@ -1023,22 +850,7 @@ procedure Net#anon$2#exit#13()
   assume (forall idx$: int :: 
     (0 <= idx$) && (idx$ < (R[Net#e] + C[Net#e])) ==> (M[Net#e][idx$] == M[Net#c][idx$])
   );
-  assume (R[Net#a] + C[Net#a]) <= 2;
-  assume (forall i: int :: 
-    (1 <= i) && (i < (R[Net#a] + C[Net#a])) ==> (M[Net#a][i] > M[Net#a][i - 1])
-  );
-  assume (forall i: int :: 
-    (1 <= i) && (i < (R[Net#b] + C[Net#b])) ==> (M[Net#b][i] > M[Net#b][i - 1])
-  );
-  assume (forall i: int :: 
-    (1 <= i) && (i < (R[Net#c] + C[Net#c])) ==> (M[Net#c][i] > M[Net#c][i - 1])
-  );
-  assume (forall i: int :: 
-    (1 <= i) && (i < (R[Net#d] + C[Net#d])) ==> (M[Net#d][i] > M[Net#d][i - 1])
-  );
-  assume (forall i: int :: 
-    (1 <= i) && (i < (R[Net#e] + C[Net#e])) ==> (M[Net#e][i] > M[Net#e][i - 1])
-  );
+  assume (R[Net#a] + C[Net#a]) <= 3;
   assume C[Net#f] == 1;
   assume C[Net#g] == R[Net#e];
   assume R[Net#e] == M[Net#f][R[Net#f]];
@@ -1056,9 +868,10 @@ procedure Net#anon$2#exit#13()
   assume !((!((1 <= C[Net#d]) && (1 <= C[Net#f]) && (M[Net#d][R[Net#d] - 0] < M[Net#f][R[Net#f] - 0]))) && (!((1 <= C[Net#d]) && (1 <= C[Net#e]) && (1 <= C[Net#f]) && (M[Net#d][R[Net#d] - 0] == M[Net#e][R[Net#e] - 0]) && (M[Net#d][R[Net#d] - 0] == M[Net#f][R[Net#f] - 0]))) && (1 <= C[Net#e]) && (1 <= C[Net#f]));
   ActionPH#y1 := M[Net#g][0];
   ActionPH#y2 := M[Net#g][1];
-  assert {:msg "  34.13: Network action postcondition might not hold"} (ActionPH#y1 == M[Net#a][0]) && (ActionPH#y2 == M[Net#a][1]);
+  ActionPH#y3 := M[Net#g][2];
+  assert {:msg "  34.13: Network action postcondition might not hold"} (ActionPH#y1 == M[Net#a][0]) && (ActionPH#y2 == M[Net#a][1]) && (ActionPH#y3 == M[Net#a][2]);
   R[Net#g] := R[Net#g] + C[Net#g];
-  C[Net#g] := C[Net#g] - (2 * Base#L);
+  C[Net#g] := C[Net#g] - (3 * Base#L);
   C[Net#f] := C[Net#f] - 1;
   assume M[Net#f][R[Net#f]] == 0;
   assert {:msg "  32.3: The network might leave unread tokens on channel a"} C[Net#a] == 0;
